platform/facade/CompileSafe.v
@@ -41,13 +41,6 @@ Section ADTValue.
 
   Notation CitoSafe := (@Semantics.Safe ADTValue).
 
-  Ltac try_eexists := try match goal with | |- exists _, _ => eexists end.
-  Ltac try_split := try match goal with | |- _ /\ _ => split end.
-  Ltac eexists_split := 
-    try match goal with
-          | |- exists _, _ => eexists
-          | |- _ /\ _ => split
-        end.
   Ltac pick_related := try match goal with | |- related _ _ => eauto end.
 
   Hint Constructors NoDup.
