platform/facade/DFacade.v
@@ -108,6 +108,7 @@ Section ADTSection.
       ret_not_in_args : negb (is_in RetVar ArgVars) = true;
       no_assign_to_args : is_disjoint (assigned Body) ArgVars = true;
       args_name_ok : forallb is_good_varname ArgVars = true;
+      ret_name_ok : is_good_varname RetVar = true;
       syntax_ok : is_syntax_ok Body = true
     }.
 
